Flatten the structure of Identifier.v
This is in preparation for autogenerating most of Identifier.v

To allow most of the code to continue compiling without much
modification, all of the qualified names we used to have in Identifier.v
now exist as only-parsing notations in API.v.

src/Fancy/Compiler.v
@@ -1,6 +1,5 @@
 Require Import Coq.ZArith.ZArith Coq.micromega.Lia.
 Require Import Coq.Lists.List. Import ListNotations.
-Require Import Crypto.Language.Identifier. Import Identifier.Compilers.
 Require Import Crypto.Language.Wf. Import Language.Wf.Compilers.
 Require Import Crypto.Language.Inversion. Import Language.Inversion.Compilers.
 Require Import Crypto.Language.API. Import Language.API.Compilers.
@@ -24,7 +23,12 @@ Local Open Scope Z_scope.
 
 (* TODO: organize this file *)
 Section of_prefancy.
-  Local Notation cexpr := (@Compilers.expr.expr base.type ident.ident).
+  (* We would like to write [Local Notation cexpr := (@API.expr).] but
+     we can't, in part because implicit status doesn't work through
+     nested notations, and in part because
+     COQBUG(https://github.com/coq/coq/issues/10803) *)
+  (* Set Printing All. Print API.expr. *)
+  Local Notation cexpr := (@expr.expr (Language.Compilers.base.type.type Compilers.base) Identifier.Compilers.ident).
   Local Notation LetInAppIdentZ S D r eidc x f
     := (expr.LetIn
           (A:=type.base (base.type.type_base base.type.Z))
@@ -269,7 +273,8 @@ Section of_prefancy.
     Definition cast_oor (r : zrange) (v : Z) := v mod (upper r + 1).
     Local Notation "'existZ' x" := (existT _ (type.base tZ) x) (at level 200).
     Local Notation "'existZZ' x" := (existT _ (type.base (tZ * tZ)%etype) x) (at level 200).
-    Local Notation cinterp := (expr.interp (@ident.gen_interp cast_oor)).
+    Local Notation cgen_interp coor := (API.gen_interp coor).
+    Local Notation cinterp := (API.gen_interp cast_oor).
     Definition interp_if_Z {t} (e : cexpr t) : option Z :=
       option_map (expr.interp (@ident.gen_interp cast_oor) (t:=tZ))
                  (type.try_transport
