src/Language/IdentifiersGENERATED.v
@@ -2,12 +2,12 @@ Require Import Crypto.Language.Identifier.
 Require Import Crypto.Language.IdentifiersGenerate.
 
 Module Compilers.
-  Export Identifier.Compilers.
+  Import Identifier.Compilers.
   Export IdentifiersGenerate.Compilers.
 
   Module pattern.
     Export IdentifiersGenerate.Compilers.pattern.
-    Notation type := (type Compilers.base.type.base).
+    Notation type := (type Compilers.base).
 
     Module Raw.
       Export IdentifiersGenerate.Compilers.pattern.Raw.
@@ -15,110 +15,110 @@ Module Compilers.
         Export IdentifiersGenerate.Compilers.pattern.Raw.ident.
         Module PrintIdent.
           Import Raw.ident.Tactics.MakeIdent.
-          Import Identifier.Compilers.ident.
+          Import Identifier.Compilers.
           Local Unset Printing Notations.
-          (*Goal True. print_ident Compilers.ident.ident. Abort.*)
+          (*Goal True. print_ident Compilers.ident. Abort.*)
         End PrintIdent.
 
         Local Unset Decidable Equality Schemes.
         Local Unset Boolean Equality Schemes.
         Inductive ident :=
-        | Literal
-        | Nat_succ
-        | Nat_pred
-        | Nat_max
-        | Nat_mul
-        | Nat_add
-        | Nat_sub
-        | Nat_eqb
-        | nil
-        | cons
-        | tt
-        | pair
-        | fst
-        | snd
-        | prod_rect
-        | bool_rect
-        | nat_rect
-        | nat_rect_arrow
-        | eager_nat_rect
-        | eager_nat_rect_arrow
-        | list_rect
-        | list_rect_arrow
-        | eager_list_rect
-        | eager_list_rect_arrow
-        | list_case
-        | List_length
-        | List_seq
-        | List_firstn
-        | List_skipn
-        | List_repeat
-        | List_combine
-        | List_map
-        | List_app
-        | List_rev
-        | List_flat_map
-        | List_partition
-        | List_fold_right
-        | List_update_nth
-        | List_nth_default
-        | eager_List_nth_default
-        | Z_add
-        | Z_mul
-        | Z_pow
-        | Z_sub
-        | Z_opp
-        | Z_div
-        | Z_modulo
-        | Z_log2
-        | Z_log2_up
-        | Z_eqb
-        | Z_leb
-        | Z_ltb
-        | Z_geb
-        | Z_gtb
-        | Z_of_nat
-        | Z_to_nat
-        | Z_shiftr
-        | Z_shiftl
-        | Z_land
-        | Z_lor
-        | Z_min
-        | Z_max
-        | Z_bneg
-        | Z_lnot_modulo
-        | Z_truncating_shiftl
-        | Z_mul_split
-        | Z_add_get_carry
-        | Z_add_with_carry
-        | Z_add_with_get_carry
-        | Z_sub_get_borrow
-        | Z_sub_with_get_borrow
-        | Z_zselect
-        | Z_add_modulo
-        | Z_rshi
-        | Z_cc_m
-        | Z_combine_at_bitwidth
-        | Z_cast
-        | Z_cast2
-        | option_Some
-        | option_None
-        | option_rect
-        | Build_zrange
-        | zrange_rect
-        | fancy_add
-        | fancy_addc
-        | fancy_sub
-        | fancy_subb
-        | fancy_mulll
-        | fancy_mullh
-        | fancy_mulhl
-        | fancy_mulhh
-        | fancy_rshi
-        | fancy_selc
-        | fancy_selm
-        | fancy_sell
-        | fancy_addm
+        | ident_Literal
+        | ident_Nat_succ
+        | ident_Nat_pred
+        | ident_Nat_max
+        | ident_Nat_mul
+        | ident_Nat_add
+        | ident_Nat_sub
+        | ident_Nat_eqb
+        | ident_nil
+        | ident_cons
+        | ident_tt
+        | ident_pair
+        | ident_fst
+        | ident_snd
+        | ident_prod_rect
+        | ident_bool_rect
+        | ident_nat_rect
+        | ident_nat_rect_arrow
+        | ident_eager_nat_rect
+        | ident_eager_nat_rect_arrow
+        | ident_list_rect
+        | ident_list_rect_arrow
+        | ident_eager_list_rect
+        | ident_eager_list_rect_arrow
+        | ident_list_case
+        | ident_List_length
+        | ident_List_seq
+        | ident_List_firstn
+        | ident_List_skipn
+        | ident_List_repeat
+        | ident_List_combine
+        | ident_List_map
+        | ident_List_app
+        | ident_List_rev
+        | ident_List_flat_map
+        | ident_List_partition
+        | ident_List_fold_right
+        | ident_List_update_nth
+        | ident_List_nth_default
+        | ident_eager_List_nth_default
+        | ident_Z_add
+        | ident_Z_mul
+        | ident_Z_pow
+        | ident_Z_sub
+        | ident_Z_opp
+        | ident_Z_div
+        | ident_Z_modulo
+        | ident_Z_log2
+        | ident_Z_log2_up
+        | ident_Z_eqb
+        | ident_Z_leb
+        | ident_Z_ltb
+        | ident_Z_geb
+        | ident_Z_gtb
+        | ident_Z_of_nat
+        | ident_Z_to_nat
+        | ident_Z_shiftr
+        | ident_Z_shiftl
+        | ident_Z_land
+        | ident_Z_lor
+        | ident_Z_min
+        | ident_Z_max
+        | ident_Z_bneg
+        | ident_Z_lnot_modulo
+        | ident_Z_truncating_shiftl
+        | ident_Z_mul_split
+        | ident_Z_add_get_carry
+        | ident_Z_add_with_carry
+        | ident_Z_add_with_get_carry
+        | ident_Z_sub_get_borrow
+        | ident_Z_sub_with_get_borrow
+        | ident_Z_zselect
+        | ident_Z_add_modulo
+        | ident_Z_rshi
+        | ident_Z_cc_m
+        | ident_Z_combine_at_bitwidth
+        | ident_Z_cast
+        | ident_Z_cast2
+        | ident_Some
+        | ident_None
+        | ident_option_rect
+        | ident_Build_zrange
+        | ident_zrange_rect
+        | ident_fancy_add
+        | ident_fancy_addc
+        | ident_fancy_sub
+        | ident_fancy_subb
+        | ident_fancy_mulll
+        | ident_fancy_mullh
+        | ident_fancy_mulhl
+        | ident_fancy_mulhh
+        | ident_fancy_rshi
+        | ident_fancy_selc
+        | ident_fancy_selm
+        | ident_fancy_sell
+        | ident_fancy_addm
         .
       End ident.
       Notation ident := ident.ident.
@@ -128,114 +128,117 @@ Module Compilers.
       Export IdentifiersGenerate.Compilers.pattern.ident.
       Module PrintIdent.
         Import ident.Tactics.PrintIdent.
-        Import Compilers.ident.
+        Import Identifier.Compilers.
+        Import Coq.Init.Datatypes.
+        Import Coq.ZArith.BinInt.
+        Import Crypto.Util.ZRange.
         Local Set Printing Coercions.
         Local Unset Printing Notations.
         Local Set Printing Width 10000.
-        (*Goal True. print_ident Compilers.ident.ident. Abort.*)
+        (*Goal True. print_ident Compilers.ident. Abort.*)
       End PrintIdent.
       Local Unset Decidable Equality Schemes.
       Inductive ident : type -> Type :=
-      | Literal : (forall t : base.type.base, ident (type.base (base.type.type_base t)))
-      | Nat_succ : (ident (type.arrow (type.base (base.type.type_base Compilers.base.type.nat)) (type.base (base.type.type_base Compilers.base.type.nat))))
-      | Nat_pred : (ident (type.arrow (type.base (base.type.type_base Compilers.base.type.nat)) (type.base (base.type.type_base Compilers.base.type.nat))))
-      | Nat_max : (ident (type.arrow (type.base (base.type.type_base Compilers.base.type.nat)) (type.arrow (type.base (base.type.type_base Compilers.base.type.nat)) (type.base (base.type.type_base Compilers.base.type.nat)))))
-      | Nat_mul : (ident (type.arrow (type.base (base.type.type_base Compilers.base.type.nat)) (type.arrow (type.base (base.type.type_base Compilers.base.type.nat)) (type.base (base.type.type_base Compilers.base.type.nat)))))
-      | Nat_add : (ident (type.arrow (type.base (base.type.type_base Compilers.base.type.nat)) (type.arrow (type.base (base.type.type_base Compilers.base.type.nat)) (type.base (base.type.type_base Compilers.base.type.nat)))))
-      | Nat_sub : (ident (type.arrow (type.base (base.type.type_base Compilers.base.type.nat)) (type.arrow (type.base (base.type.type_base Compilers.base.type.nat)) (type.base (base.type.type_base Compilers.base.type.nat)))))
-      | Nat_eqb : (ident (type.arrow (type.base (base.type.type_base Compilers.base.type.nat)) (type.arrow (type.base (base.type.type_base Compilers.base.type.nat)) (type.base (base.type.type_base base.type.bool)))))
-      | nil : (forall t : base.type.type base.type.base, ident (type.base (base.type.list t)))
-      | cons : (forall t : base.type.type base.type.base, ident (type.arrow (type.base t) (type.arrow (type.base (base.type.list t)) (type.base (base.type.list t)))))
-      | tt : (ident (type.base base.type.unit))
-      | pair : (forall A B : base.type.type base.type.base, ident (type.arrow (type.base A) (type.arrow (type.base B) (type.base (base.type.prod A B)))))
-      | fst : (forall A B : base.type.type base.type.base, ident (type.arrow (type.base (base.type.prod A B)) (type.base A)))
-      | snd : (forall A B : base.type.type base.type.base, ident (type.arrow (type.base (base.type.prod A B)) (type.base B)))
-      | prod_rect : (forall A B T : base.type.type base.type.base, ident (type.arrow (type.arrow (type.base A) (type.arrow (type.base B) (type.base T))) (type.arrow (type.base (base.type.prod A B)) (type.base T))))
-      | bool_rect : (forall T : base.type.type base.type.base, ident (type.arrow (type.arrow (type.base base.type.unit) (type.base T)) (type.arrow (type.arrow (type.base base.type.unit) (type.base T)) (type.arrow (type.base (base.type.type_base base.type.bool)) (type.base T)))))
-      | nat_rect : (forall P : base.type.type base.type.base, ident (type.arrow (type.arrow (type.base base.type.unit) (type.base P)) (type.arrow (type.arrow (type.base (base.type.type_base Compilers.base.type.nat)) (type.arrow (type.base P) (type.base P))) (type.arrow (type.base (base.type.type_base Compilers.base.type.nat)) (type.base P)))))
-      | nat_rect_arrow : (forall P Q : base.type.type base.type.base, ident (type.arrow (type.arrow (type.base P) (type.base Q)) (type.arrow (type.arrow (type.base (base.type.type_base Compilers.base.type.nat)) (type.arrow (type.arrow (type.base P) (type.base Q)) (type.arrow (type.base P) (type.base Q)))) (type.arrow (type.base (base.type.type_base Compilers.base.type.nat)) (type.arrow (type.base P) (type.base Q))))))
-      | eager_nat_rect : (forall P : base.type.type base.type.base, ident (type.arrow (type.arrow (type.base base.type.unit) (type.base P)) (type.arrow (type.arrow (type.base (base.type.type_base Compilers.base.type.nat)) (type.arrow (type.base P) (type.base P))) (type.arrow (type.base (base.type.type_base Compilers.base.type.nat)) (type.base P)))))
-      | eager_nat_rect_arrow : (forall P Q : base.type.type base.type.base, ident (type.arrow (type.arrow (type.base P) (type.base Q)) (type.arrow (type.arrow (type.base (base.type.type_base Compilers.base.type.nat)) (type.arrow (type.arrow (type.base P) (type.base Q)) (type.arrow (type.base P) (type.base Q)))) (type.arrow (type.base (base.type.type_base Compilers.base.type.nat)) (type.arrow (type.base P) (type.base Q))))))
-      | list_rect : (forall A P : base.type.type base.type.base, ident (type.arrow (type.arrow (type.base base.type.unit) (type.base P)) (type.arrow (type.arrow (type.base A) (type.arrow (type.base (base.type.list A)) (type.arrow (type.base P) (type.base P)))) (type.arrow (type.base (base.type.list A)) (type.base P)))))
-      | list_rect_arrow : (forall A P Q : base.type.type base.type.base, ident (type.arrow (type.arrow (type.base P) (type.base Q)) (type.arrow (type.arrow (type.base A) (type.arrow (type.base (base.type.list A)) (type.arrow (type.arrow (type.base P) (type.base Q)) (type.arrow (type.base P) (type.base Q))))) (type.arrow (type.base (base.type.list A)) (type.arrow (type.base P) (type.base Q))))))
-      | eager_list_rect : (forall A P : base.type.type base.type.base, ident (type.arrow (type.arrow (type.base base.type.unit) (type.base P)) (type.arrow (type.arrow (type.base A) (type.arrow (type.base (base.type.list A)) (type.arrow (type.base P) (type.base P)))) (type.arrow (type.base (base.type.list A)) (type.base P)))))
-      | eager_list_rect_arrow : (forall A P Q : base.type.type base.type.base, ident (type.arrow (type.arrow (type.base P) (type.base Q)) (type.arrow (type.arrow (type.base A) (type.arrow (type.base (base.type.list A)) (type.arrow (type.arrow (type.base P) (type.base Q)) (type.arrow (type.base P) (type.base Q))))) (type.arrow (type.base (base.type.list A)) (type.arrow (type.base P) (type.base Q))))))
-      | list_case : (forall A P : base.type.type base.type.base, ident (type.arrow (type.arrow (type.base base.type.unit) (type.base P)) (type.arrow (type.arrow (type.base A) (type.arrow (type.base (base.type.list A)) (type.base P))) (type.arrow (type.base (base.type.list A)) (type.base P)))))
-      | List_length : (forall T : base.type.type base.type.base, ident (type.arrow (type.base (base.type.list T)) (type.base (base.type.type_base Compilers.base.type.nat))))
-      | List_seq : (ident (type.arrow (type.base (base.type.type_base Compilers.base.type.nat)) (type.arrow (type.base (base.type.type_base Compilers.base.type.nat)) (type.base (base.type.list (base.type.type_base Compilers.base.type.nat))))))
-      | List_firstn : (forall A : base.type.type base.type.base, ident (type.arrow (type.base (base.type.type_base Compilers.base.type.nat)) (type.arrow (type.base (base.type.list A)) (type.base (base.type.list A)))))
-      | List_skipn : (forall A : base.type.type base.type.base, ident (type.arrow (type.base (base.type.type_base Compilers.base.type.nat)) (type.arrow (type.base (base.type.list A)) (type.base (base.type.list A)))))
-      | List_repeat : (forall A : base.type.type base.type.base, ident (type.arrow (type.base A) (type.arrow (type.base (base.type.type_base Compilers.base.type.nat)) (type.base (base.type.list A)))))
-      | List_combine : (forall A B : base.type.type base.type.base, ident (type.arrow (type.base (base.type.list A)) (type.arrow (type.base (base.type.list B)) (type.base (base.type.list (base.type.prod A B))))))
-      | List_map : (forall A B : base.type.type base.type.base, ident (type.arrow (type.arrow (type.base A) (type.base B)) (type.arrow (type.base (base.type.list A)) (type.base (base.type.list B)))))
-      | List_app : (forall A : base.type.type base.type.base, ident (type.arrow (type.base (base.type.list A)) (type.arrow (type.base (base.type.list A)) (type.base (base.type.list A)))))
-      | List_rev : (forall A : base.type.type base.type.base, ident (type.arrow (type.base (base.type.list A)) (type.base (base.type.list A))))
-      | List_flat_map : (forall A B : base.type.type base.type.base, ident (type.arrow (type.arrow (type.base A) (type.base (base.type.list B))) (type.arrow (type.base (base.type.list A)) (type.base (base.type.list B)))))
-      | List_partition : (forall A : base.type.type base.type.base, ident (type.arrow (type.arrow (type.base A) (type.base (base.type.type_base base.type.bool))) (type.arrow (type.base (base.type.list A)) (type.base (base.type.prod (base.type.list A) (base.type.list A))))))
-      | List_fold_right : (forall A B : base.type.type base.type.base, ident (type.arrow (type.arrow (type.base B) (type.arrow (type.base A) (type.base A))) (type.arrow (type.base A) (type.arrow (type.base (base.type.list B)) (type.base A)))))
-      | List_update_nth : (forall T : base.type.type base.type.base, ident (type.arrow (type.base (base.type.type_base Compilers.base.type.nat)) (type.arrow (type.arrow (type.base T) (type.base T)) (type.arrow (type.base (base.type.list T)) (type.base (base.type.list T))))))
-      | List_nth_default : (forall T : base.type.type base.type.base, ident (type.arrow (type.base T) (type.arrow (type.base (base.type.list T)) (type.arrow (type.base (base.type.type_base Compilers.base.type.nat)) (type.base T)))))
-      | eager_List_nth_default : (forall T : base.type.type base.type.base, ident (type.arrow (type.base T) (type.arrow (type.base (base.type.list T)) (type.arrow (type.base (base.type.type_base Compilers.base.type.nat)) (type.base T)))))
-      | Z_add : (ident (type.arrow (type.base (base.type.type_base base.type.Z)) (type.arrow (type.base (base.type.type_base base.type.Z)) (type.base (base.type.type_base base.type.Z)))))
-      | Z_mul : (ident (type.arrow (type.base (base.type.type_base base.type.Z)) (type.arrow (type.base (base.type.type_base base.type.Z)) (type.base (base.type.type_base base.type.Z)))))
-      | Z_pow : (ident (type.arrow (type.base (base.type.type_base base.type.Z)) (type.arrow (type.base (base.type.type_base base.type.Z)) (type.base (base.type.type_base base.type.Z)))))
-      | Z_sub : (ident (type.arrow (type.base (base.type.type_base base.type.Z)) (type.arrow (type.base (base.type.type_base base.type.Z)) (type.base (base.type.type_base base.type.Z)))))
-      | Z_opp : (ident (type.arrow (type.base (base.type.type_base base.type.Z)) (type.base (base.type.type_base base.type.Z))))
-      | Z_div : (ident (type.arrow (type.base (base.type.type_base base.type.Z)) (type.arrow (type.base (base.type.type_base base.type.Z)) (type.base (base.type.type_base base.type.Z)))))
-      | Z_modulo : (ident (type.arrow (type.base (base.type.type_base base.type.Z)) (type.arrow (type.base (base.type.type_base base.type.Z)) (type.base (base.type.type_base base.type.Z)))))
-      | Z_log2 : (ident (type.arrow (type.base (base.type.type_base base.type.Z)) (type.base (base.type.type_base base.type.Z))))
-      | Z_log2_up : (ident (type.arrow (type.base (base.type.type_base base.type.Z)) (type.base (base.type.type_base base.type.Z))))
-      | Z_eqb : (ident (type.arrow (type.base (base.type.type_base base.type.Z)) (type.arrow (type.base (base.type.type_base base.type.Z)) (type.base (base.type.type_base base.type.bool)))))
-      | Z_leb : (ident (type.arrow (type.base (base.type.type_base base.type.Z)) (type.arrow (type.base (base.type.type_base base.type.Z)) (type.base (base.type.type_base base.type.bool)))))
-      | Z_ltb : (ident (type.arrow (type.base (base.type.type_base base.type.Z)) (type.arrow (type.base (base.type.type_base base.type.Z)) (type.base (base.type.type_base base.type.bool)))))
-      | Z_geb : (ident (type.arrow (type.base (base.type.type_base base.type.Z)) (type.arrow (type.base (base.type.type_base base.type.Z)) (type.base (base.type.type_base base.type.bool)))))
-      | Z_gtb : (ident (type.arrow (type.base (base.type.type_base base.type.Z)) (type.arrow (type.base (base.type.type_base base.type.Z)) (type.base (base.type.type_base base.type.bool)))))
-      | Z_of_nat : (ident (type.arrow (type.base (base.type.type_base Compilers.base.type.nat)) (type.base (base.type.type_base base.type.Z))))
-      | Z_to_nat : (ident (type.arrow (type.base (base.type.type_base base.type.Z)) (type.base (base.type.type_base Compilers.base.type.nat))))
-      | Z_shiftr : (ident (type.arrow (type.base (base.type.type_base base.type.Z)) (type.arrow (type.base (base.type.type_base base.type.Z)) (type.base (base.type.type_base base.type.Z)))))
-      | Z_shiftl : (ident (type.arrow (type.base (base.type.type_base base.type.Z)) (type.arrow (type.base (base.type.type_base base.type.Z)) (type.base (base.type.type_base base.type.Z)))))
-      | Z_land : (ident (type.arrow (type.base (base.type.type_base base.type.Z)) (type.arrow (type.base (base.type.type_base base.type.Z)) (type.base (base.type.type_base base.type.Z)))))
-      | Z_lor : (ident (type.arrow (type.base (base.type.type_base base.type.Z)) (type.arrow (type.base (base.type.type_base base.type.Z)) (type.base (base.type.type_base base.type.Z)))))
-      | Z_min : (ident (type.arrow (type.base (base.type.type_base base.type.Z)) (type.arrow (type.base (base.type.type_base base.type.Z)) (type.base (base.type.type_base base.type.Z)))))
-      | Z_max : (ident (type.arrow (type.base (base.type.type_base base.type.Z)) (type.arrow (type.base (base.type.type_base base.type.Z)) (type.base (base.type.type_base base.type.Z)))))
-      | Z_bneg : (ident (type.arrow (type.base (base.type.type_base base.type.Z)) (type.base (base.type.type_base base.type.Z))))
-      | Z_lnot_modulo : (ident (type.arrow (type.base (base.type.type_base base.type.Z)) (type.arrow (type.base (base.type.type_base base.type.Z)) (type.base (base.type.type_base base.type.Z)))))
-      | Z_truncating_shiftl : (ident (type.arrow (type.base (base.type.type_base base.type.Z)) (type.arrow (type.base (base.type.type_base base.type.Z)) (type.arrow (type.base (base.type.type_base base.type.Z)) (type.base (base.type.type_base base.type.Z))))))
-      | Z_mul_split : (ident (type.arrow (type.base (base.type.type_base base.type.Z)) (type.arrow (type.base (base.type.type_base base.type.Z)) (type.arrow (type.base (base.type.type_base base.type.Z)) (type.base (base.type.prod (base.type.type_base base.type.Z) (base.type.type_base base.type.Z)))))))
-      | Z_add_get_carry : (ident (type.arrow (type.base (base.type.type_base base.type.Z)) (type.arrow (type.base (base.type.type_base base.type.Z)) (type.arrow (type.base (base.type.type_base base.type.Z)) (type.base (base.type.prod (base.type.type_base base.type.Z) (base.type.type_base base.type.Z)))))))
-      | Z_add_with_carry : (ident (type.arrow (type.base (base.type.type_base base.type.Z)) (type.arrow (type.base (base.type.type_base base.type.Z)) (type.arrow (type.base (base.type.type_base base.type.Z)) (type.base (base.type.type_base base.type.Z))))))
-      | Z_add_with_get_carry : (ident (type.arrow (type.base (base.type.type_base base.type.Z)) (type.arrow (type.base (base.type.type_base base.type.Z)) (type.arrow (type.base (base.type.type_base base.type.Z)) (type.arrow (type.base (base.type.type_base base.type.Z)) (type.base (base.type.prod (base.type.type_base base.type.Z) (base.type.type_base base.type.Z))))))))
-      | Z_sub_get_borrow : (ident (type.arrow (type.base (base.type.type_base base.type.Z)) (type.arrow (type.base (base.type.type_base base.type.Z)) (type.arrow (type.base (base.type.type_base base.type.Z)) (type.base (base.type.prod (base.type.type_base base.type.Z) (base.type.type_base base.type.Z)))))))
-      | Z_sub_with_get_borrow : (ident (type.arrow (type.base (base.type.type_base base.type.Z)) (type.arrow (type.base (base.type.type_base base.type.Z)) (type.arrow (type.base (base.type.type_base base.type.Z)) (type.arrow (type.base (base.type.type_base base.type.Z)) (type.base (base.type.prod (base.type.type_base base.type.Z) (base.type.type_base base.type.Z))))))))
-      | Z_zselect : (ident (type.arrow (type.base (base.type.type_base base.type.Z)) (type.arrow (type.base (base.type.type_base base.type.Z)) (type.arrow (type.base (base.type.type_base base.type.Z)) (type.base (base.type.type_base base.type.Z))))))
-      | Z_add_modulo : (ident (type.arrow (type.base (base.type.type_base base.type.Z)) (type.arrow (type.base (base.type.type_base base.type.Z)) (type.arrow (type.base (base.type.type_base base.type.Z)) (type.base (base.type.type_base base.type.Z))))))
-      | Z_rshi : (ident (type.arrow (type.base (base.type.type_base base.type.Z)) (type.arrow (type.base (base.type.type_base base.type.Z)) (type.arrow (type.base (base.type.type_base base.type.Z)) (type.arrow (type.base (base.type.type_base base.type.Z)) (type.base (base.type.type_base base.type.Z)))))))
-      | Z_cc_m : (ident (type.arrow (type.base (base.type.type_base base.type.Z)) (type.arrow (type.base (base.type.type_base base.type.Z)) (type.base (base.type.type_base base.type.Z)))))
-      | Z_combine_at_bitwidth : (ident (type.arrow (type.base (base.type.type_base base.type.Z)) (type.arrow (type.base (base.type.type_base base.type.Z)) (type.arrow (type.base (base.type.type_base base.type.Z)) (type.base (base.type.type_base base.type.Z))))))
-      | Z_cast : (ident (type.arrow (type.base (base.type.type_base base.type.Z)) (type.base (base.type.type_base base.type.Z))))
-      | Z_cast2 : (ident (type.arrow (type.base (base.type.prod (base.type.type_base base.type.Z) (base.type.type_base base.type.Z))) (type.base (base.type.prod (base.type.type_base base.type.Z) (base.type.type_base base.type.Z)))))
-      | option_Some : (forall A : base.type.type base.type.base, ident (type.arrow (type.base A) (type.base (base.type.option A))))
-      | option_None : (forall A : base.type.type base.type.base, ident (type.base (base.type.option A)))
-      | option_rect : (forall A P : base.type.type base.type.base, ident (type.arrow (type.arrow (type.base A) (type.base P)) (type.arrow (type.arrow (type.base base.type.unit) (type.base P)) (type.arrow (type.base (base.type.option A)) (type.base P)))))
-      | Build_zrange : (ident (type.arrow (type.base (base.type.type_base base.type.Z)) (type.arrow (type.base (base.type.type_base base.type.Z)) (type.base (base.type.type_base base.type.zrange)))))
-      | zrange_rect : (forall P : base.type.type base.type.base, ident (type.arrow (type.arrow (type.base (base.type.type_base base.type.Z)) (type.arrow (type.base (base.type.type_base base.type.Z)) (type.base P))) (type.arrow (type.base (base.type.type_base base.type.zrange)) (type.base P))))
-      | fancy_add : (ident (type.arrow (type.base (base.type.prod (base.type.prod (base.type.type_base base.type.Z) (base.type.type_base base.type.Z)) (base.type.prod (base.type.type_base base.type.Z) (base.type.type_base base.type.Z)))) (type.base (base.type.prod (base.type.type_base base.type.Z) (base.type.type_base base.type.Z)))))
-      | fancy_addc : (ident (type.arrow (type.base (base.type.prod (base.type.prod (base.type.type_base base.type.Z) (base.type.type_base base.type.Z)) (base.type.prod (base.type.prod (base.type.type_base base.type.Z) (base.type.type_base base.type.Z)) (base.type.type_base base.type.Z)))) (type.base (base.type.prod (base.type.type_base base.type.Z) (base.type.type_base base.type.Z)))))
-      | fancy_sub : (ident (type.arrow (type.base (base.type.prod (base.type.prod (base.type.type_base base.type.Z) (base.type.type_base base.type.Z)) (base.type.prod (base.type.type_base base.type.Z) (base.type.type_base base.type.Z)))) (type.base (base.type.prod (base.type.type_base base.type.Z) (base.type.type_base base.type.Z)))))
-      | fancy_subb : (ident (type.arrow (type.base (base.type.prod (base.type.prod (base.type.type_base base.type.Z) (base.type.type_base base.type.Z)) (base.type.prod (base.type.prod (base.type.type_base base.type.Z) (base.type.type_base base.type.Z)) (base.type.type_base base.type.Z)))) (type.base (base.type.prod (base.type.type_base base.type.Z) (base.type.type_base base.type.Z)))))
-      | fancy_mulll : (ident (type.arrow (type.base (base.type.prod (base.type.type_base base.type.Z) (base.type.prod (base.type.type_base base.type.Z) (base.type.type_base base.type.Z)))) (type.base (base.type.type_base base.type.Z))))
-      | fancy_mullh : (ident (type.arrow (type.base (base.type.prod (base.type.type_base base.type.Z) (base.type.prod (base.type.type_base base.type.Z) (base.type.type_base base.type.Z)))) (type.base (base.type.type_base base.type.Z))))
-      | fancy_mulhl : (ident (type.arrow (type.base (base.type.prod (base.type.type_base base.type.Z) (base.type.prod (base.type.type_base base.type.Z) (base.type.type_base base.type.Z)))) (type.base (base.type.type_base base.type.Z))))
-      | fancy_mulhh : (ident (type.arrow (type.base (base.type.prod (base.type.type_base base.type.Z) (base.type.prod (base.type.type_base base.type.Z) (base.type.type_base base.type.Z)))) (type.base (base.type.type_base base.type.Z))))
-      | fancy_rshi : (ident (type.arrow (type.base (base.type.prod (base.type.prod (base.type.type_base base.type.Z) (base.type.type_base base.type.Z)) (base.type.prod (base.type.type_base base.type.Z) (base.type.type_base base.type.Z)))) (type.base (base.type.type_base base.type.Z))))
-      | fancy_selc : (ident (type.arrow (type.base (base.type.prod (base.type.prod (base.type.type_base base.type.Z) (base.type.type_base base.type.Z)) (base.type.type_base base.type.Z))) (type.base (base.type.type_base base.type.Z))))
-      | fancy_selm : (ident (type.arrow (type.base (base.type.prod (base.type.type_base base.type.Z) (base.type.prod (base.type.prod (base.type.type_base base.type.Z) (base.type.type_base base.type.Z)) (base.type.type_base base.type.Z)))) (type.base (base.type.type_base base.type.Z))))
-      | fancy_sell : (ident (type.arrow (type.base (base.type.prod (base.type.prod (base.type.type_base base.type.Z) (base.type.type_base base.type.Z)) (base.type.type_base base.type.Z))) (type.base (base.type.type_base base.type.Z))))
-      | fancy_addm : (ident (type.arrow (type.base (base.type.prod (base.type.prod (base.type.type_base base.type.Z) (base.type.type_base base.type.Z)) (base.type.type_base base.type.Z))) (type.base (base.type.type_base base.type.Z))))
+      | ident_Literal : (forall t : base, ident (type.base (pattern.base.type.type_base t)))
+      | ident_Nat_succ : (ident (type.arrow (type.base (pattern.base.type.type_base Compilers.nat)) (type.base (pattern.base.type.type_base Compilers.nat))))
+      | ident_Nat_pred : (ident (type.arrow (type.base (pattern.base.type.type_base Compilers.nat)) (type.base (pattern.base.type.type_base Compilers.nat))))
+      | ident_Nat_max : (ident (type.arrow (type.base (pattern.base.type.type_base Compilers.nat)) (type.arrow (type.base (pattern.base.type.type_base Compilers.nat)) (type.base (pattern.base.type.type_base Compilers.nat)))))
+      | ident_Nat_mul : (ident (type.arrow (type.base (pattern.base.type.type_base Compilers.nat)) (type.arrow (type.base (pattern.base.type.type_base Compilers.nat)) (type.base (pattern.base.type.type_base Compilers.nat)))))
+      | ident_Nat_add : (ident (type.arrow (type.base (pattern.base.type.type_base Compilers.nat)) (type.arrow (type.base (pattern.base.type.type_base Compilers.nat)) (type.base (pattern.base.type.type_base Compilers.nat)))))
+      | ident_Nat_sub : (ident (type.arrow (type.base (pattern.base.type.type_base Compilers.nat)) (type.arrow (type.base (pattern.base.type.type_base Compilers.nat)) (type.base (pattern.base.type.type_base Compilers.nat)))))
+      | ident_Nat_eqb : (ident (type.arrow (type.base (pattern.base.type.type_base Compilers.nat)) (type.arrow (type.base (pattern.base.type.type_base Compilers.nat)) (type.base (pattern.base.type.type_base Compilers.bool)))))
+      | ident_nil : (forall t : pattern.base.type.type base, ident (type.base (pattern.base.type.list t)))
+      | ident_cons : (forall t : pattern.base.type.type base, ident (type.arrow (type.base t) (type.arrow (type.base (pattern.base.type.list t)) (type.base (pattern.base.type.list t)))))
+      | ident_tt : (ident (type.base pattern.base.type.unit))
+      | ident_pair : (forall A B : pattern.base.type.type base, ident (type.arrow (type.base A) (type.arrow (type.base B) (type.base (pattern.base.type.prod A B)))))
+      | ident_fst : (forall A B : pattern.base.type.type base, ident (type.arrow (type.base (pattern.base.type.prod A B)) (type.base A)))
+      | ident_snd : (forall A B : pattern.base.type.type base, ident (type.arrow (type.base (pattern.base.type.prod A B)) (type.base B)))
+      | ident_prod_rect : (forall A B T : pattern.base.type.type base, ident (type.arrow (type.arrow (type.base A) (type.arrow (type.base B) (type.base T))) (type.arrow (type.base (pattern.base.type.prod A B)) (type.base T))))
+      | ident_bool_rect : (forall T : pattern.base.type.type base, ident (type.arrow (type.arrow (type.base pattern.base.type.unit) (type.base T)) (type.arrow (type.arrow (type.base pattern.base.type.unit) (type.base T)) (type.arrow (type.base (pattern.base.type.type_base Compilers.bool)) (type.base T)))))
+      | ident_nat_rect : (forall P : pattern.base.type.type base, ident (type.arrow (type.arrow (type.base pattern.base.type.unit) (type.base P)) (type.arrow (type.arrow (type.base (pattern.base.type.type_base Compilers.nat)) (type.arrow (type.base P) (type.base P))) (type.arrow (type.base (pattern.base.type.type_base Compilers.nat)) (type.base P)))))
+      | ident_nat_rect_arrow : (forall P Q : pattern.base.type.type base, ident (type.arrow (type.arrow (type.base P) (type.base Q)) (type.arrow (type.arrow (type.base (pattern.base.type.type_base Compilers.nat)) (type.arrow (type.arrow (type.base P) (type.base Q)) (type.arrow (type.base P) (type.base Q)))) (type.arrow (type.base (pattern.base.type.type_base Compilers.nat)) (type.arrow (type.base P) (type.base Q))))))
+      | ident_eager_nat_rect : (forall P : pattern.base.type.type base, ident (type.arrow (type.arrow (type.base pattern.base.type.unit) (type.base P)) (type.arrow (type.arrow (type.base (pattern.base.type.type_base Compilers.nat)) (type.arrow (type.base P) (type.base P))) (type.arrow (type.base (pattern.base.type.type_base Compilers.nat)) (type.base P)))))
+      | ident_eager_nat_rect_arrow : (forall P Q : pattern.base.type.type base, ident (type.arrow (type.arrow (type.base P) (type.base Q)) (type.arrow (type.arrow (type.base (pattern.base.type.type_base Compilers.nat)) (type.arrow (type.arrow (type.base P) (type.base Q)) (type.arrow (type.base P) (type.base Q)))) (type.arrow (type.base (pattern.base.type.type_base Compilers.nat)) (type.arrow (type.base P) (type.base Q))))))
+      | ident_list_rect : (forall A P : pattern.base.type.type base, ident (type.arrow (type.arrow (type.base pattern.base.type.unit) (type.base P)) (type.arrow (type.arrow (type.base A) (type.arrow (type.base (pattern.base.type.list A)) (type.arrow (type.base P) (type.base P)))) (type.arrow (type.base (pattern.base.type.list A)) (type.base P)))))
+      | ident_list_rect_arrow : (forall A P Q : pattern.base.type.type base, ident (type.arrow (type.arrow (type.base P) (type.base Q)) (type.arrow (type.arrow (type.base A) (type.arrow (type.base (pattern.base.type.list A)) (type.arrow (type.arrow (type.base P) (type.base Q)) (type.arrow (type.base P) (type.base Q))))) (type.arrow (type.base (pattern.base.type.list A)) (type.arrow (type.base P) (type.base Q))))))
+      | ident_eager_list_rect : (forall A P : pattern.base.type.type base, ident (type.arrow (type.arrow (type.base pattern.base.type.unit) (type.base P)) (type.arrow (type.arrow (type.base A) (type.arrow (type.base (pattern.base.type.list A)) (type.arrow (type.base P) (type.base P)))) (type.arrow (type.base (pattern.base.type.list A)) (type.base P)))))
+      | ident_eager_list_rect_arrow : (forall A P Q : pattern.base.type.type base, ident (type.arrow (type.arrow (type.base P) (type.base Q)) (type.arrow (type.arrow (type.base A) (type.arrow (type.base (pattern.base.type.list A)) (type.arrow (type.arrow (type.base P) (type.base Q)) (type.arrow (type.base P) (type.base Q))))) (type.arrow (type.base (pattern.base.type.list A)) (type.arrow (type.base P) (type.base Q))))))
+      | ident_list_case : (forall A P : pattern.base.type.type base, ident (type.arrow (type.arrow (type.base pattern.base.type.unit) (type.base P)) (type.arrow (type.arrow (type.base A) (type.arrow (type.base (pattern.base.type.list A)) (type.base P))) (type.arrow (type.base (pattern.base.type.list A)) (type.base P)))))
+      | ident_List_length : (forall T : pattern.base.type.type base, ident (type.arrow (type.base (pattern.base.type.list T)) (type.base (pattern.base.type.type_base Compilers.nat))))
+      | ident_List_seq : (ident (type.arrow (type.base (pattern.base.type.type_base Compilers.nat)) (type.arrow (type.base (pattern.base.type.type_base Compilers.nat)) (type.base (pattern.base.type.list (pattern.base.type.type_base Compilers.nat))))))
+      | ident_List_firstn : (forall A : pattern.base.type.type base, ident (type.arrow (type.base (pattern.base.type.type_base Compilers.nat)) (type.arrow (type.base (pattern.base.type.list A)) (type.base (pattern.base.type.list A)))))
+      | ident_List_skipn : (forall A : pattern.base.type.type base, ident (type.arrow (type.base (pattern.base.type.type_base Compilers.nat)) (type.arrow (type.base (pattern.base.type.list A)) (type.base (pattern.base.type.list A)))))
+      | ident_List_repeat : (forall A : pattern.base.type.type base, ident (type.arrow (type.base A) (type.arrow (type.base (pattern.base.type.type_base Compilers.nat)) (type.base (pattern.base.type.list A)))))
+      | ident_List_combine : (forall A B : pattern.base.type.type base, ident (type.arrow (type.base (pattern.base.type.list A)) (type.arrow (type.base (pattern.base.type.list B)) (type.base (pattern.base.type.list (pattern.base.type.prod A B))))))
+      | ident_List_map : (forall A B : pattern.base.type.type base, ident (type.arrow (type.arrow (type.base A) (type.base B)) (type.arrow (type.base (pattern.base.type.list A)) (type.base (pattern.base.type.list B)))))
+      | ident_List_app : (forall A : pattern.base.type.type base, ident (type.arrow (type.base (pattern.base.type.list A)) (type.arrow (type.base (pattern.base.type.list A)) (type.base (pattern.base.type.list A)))))
+      | ident_List_rev : (forall A : pattern.base.type.type base, ident (type.arrow (type.base (pattern.base.type.list A)) (type.base (pattern.base.type.list A))))
+      | ident_List_flat_map : (forall A B : pattern.base.type.type base, ident (type.arrow (type.arrow (type.base A) (type.base (pattern.base.type.list B))) (type.arrow (type.base (pattern.base.type.list A)) (type.base (pattern.base.type.list B)))))
+      | ident_List_partition : (forall A : pattern.base.type.type base, ident (type.arrow (type.arrow (type.base A) (type.base (pattern.base.type.type_base Compilers.bool))) (type.arrow (type.base (pattern.base.type.list A)) (type.base (pattern.base.type.prod (pattern.base.type.list A) (pattern.base.type.list A))))))
+      | ident_List_fold_right : (forall A B : pattern.base.type.type base, ident (type.arrow (type.arrow (type.base B) (type.arrow (type.base A) (type.base A))) (type.arrow (type.base A) (type.arrow (type.base (pattern.base.type.list B)) (type.base A)))))
+      | ident_List_update_nth : (forall T : pattern.base.type.type base, ident (type.arrow (type.base (pattern.base.type.type_base Compilers.nat)) (type.arrow (type.arrow (type.base T) (type.base T)) (type.arrow (type.base (pattern.base.type.list T)) (type.base (pattern.base.type.list T))))))
+      | ident_List_nth_default : (forall T : pattern.base.type.type base, ident (type.arrow (type.base T) (type.arrow (type.base (pattern.base.type.list T)) (type.arrow (type.base (pattern.base.type.type_base Compilers.nat)) (type.base T)))))
+      | ident_eager_List_nth_default : (forall T : pattern.base.type.type base, ident (type.arrow (type.base T) (type.arrow (type.base (pattern.base.type.list T)) (type.arrow (type.base (pattern.base.type.type_base Compilers.nat)) (type.base T)))))
+      | ident_Z_add : (ident (type.arrow (type.base (pattern.base.type.type_base Compilers.Z)) (type.arrow (type.base (pattern.base.type.type_base Compilers.Z)) (type.base (pattern.base.type.type_base Compilers.Z)))))
+      | ident_Z_mul : (ident (type.arrow (type.base (pattern.base.type.type_base Compilers.Z)) (type.arrow (type.base (pattern.base.type.type_base Compilers.Z)) (type.base (pattern.base.type.type_base Compilers.Z)))))
+      | ident_Z_pow : (ident (type.arrow (type.base (pattern.base.type.type_base Compilers.Z)) (type.arrow (type.base (pattern.base.type.type_base Compilers.Z)) (type.base (pattern.base.type.type_base Compilers.Z)))))
+      | ident_Z_sub : (ident (type.arrow (type.base (pattern.base.type.type_base Compilers.Z)) (type.arrow (type.base (pattern.base.type.type_base Compilers.Z)) (type.base (pattern.base.type.type_base Compilers.Z)))))
+      | ident_Z_opp : (ident (type.arrow (type.base (pattern.base.type.type_base Compilers.Z)) (type.base (pattern.base.type.type_base Compilers.Z))))
+      | ident_Z_div : (ident (type.arrow (type.base (pattern.base.type.type_base Compilers.Z)) (type.arrow (type.base (pattern.base.type.type_base Compilers.Z)) (type.base (pattern.base.type.type_base Compilers.Z)))))
+      | ident_Z_modulo : (ident (type.arrow (type.base (pattern.base.type.type_base Compilers.Z)) (type.arrow (type.base (pattern.base.type.type_base Compilers.Z)) (type.base (pattern.base.type.type_base Compilers.Z)))))
+      | ident_Z_log2 : (ident (type.arrow (type.base (pattern.base.type.type_base Compilers.Z)) (type.base (pattern.base.type.type_base Compilers.Z))))
+      | ident_Z_log2_up : (ident (type.arrow (type.base (pattern.base.type.type_base Compilers.Z)) (type.base (pattern.base.type.type_base Compilers.Z))))
+      | ident_Z_eqb : (ident (type.arrow (type.base (pattern.base.type.type_base Compilers.Z)) (type.arrow (type.base (pattern.base.type.type_base Compilers.Z)) (type.base (pattern.base.type.type_base Compilers.bool)))))
+      | ident_Z_leb : (ident (type.arrow (type.base (pattern.base.type.type_base Compilers.Z)) (type.arrow (type.base (pattern.base.type.type_base Compilers.Z)) (type.base (pattern.base.type.type_base Compilers.bool)))))
+      | ident_Z_ltb : (ident (type.arrow (type.base (pattern.base.type.type_base Compilers.Z)) (type.arrow (type.base (pattern.base.type.type_base Compilers.Z)) (type.base (pattern.base.type.type_base Compilers.bool)))))
+      | ident_Z_geb : (ident (type.arrow (type.base (pattern.base.type.type_base Compilers.Z)) (type.arrow (type.base (pattern.base.type.type_base Compilers.Z)) (type.base (pattern.base.type.type_base Compilers.bool)))))
+      | ident_Z_gtb : (ident (type.arrow (type.base (pattern.base.type.type_base Compilers.Z)) (type.arrow (type.base (pattern.base.type.type_base Compilers.Z)) (type.base (pattern.base.type.type_base Compilers.bool)))))
+      | ident_Z_of_nat : (ident (type.arrow (type.base (pattern.base.type.type_base Compilers.nat)) (type.base (pattern.base.type.type_base Compilers.Z))))
+      | ident_Z_to_nat : (ident (type.arrow (type.base (pattern.base.type.type_base Compilers.Z)) (type.base (pattern.base.type.type_base Compilers.nat))))
+      | ident_Z_shiftr : (ident (type.arrow (type.base (pattern.base.type.type_base Compilers.Z)) (type.arrow (type.base (pattern.base.type.type_base Compilers.Z)) (type.base (pattern.base.type.type_base Compilers.Z)))))
+      | ident_Z_shiftl : (ident (type.arrow (type.base (pattern.base.type.type_base Compilers.Z)) (type.arrow (type.base (pattern.base.type.type_base Compilers.Z)) (type.base (pattern.base.type.type_base Compilers.Z)))))
+      | ident_Z_land : (ident (type.arrow (type.base (pattern.base.type.type_base Compilers.Z)) (type.arrow (type.base (pattern.base.type.type_base Compilers.Z)) (type.base (pattern.base.type.type_base Compilers.Z)))))
+      | ident_Z_lor : (ident (type.arrow (type.base (pattern.base.type.type_base Compilers.Z)) (type.arrow (type.base (pattern.base.type.type_base Compilers.Z)) (type.base (pattern.base.type.type_base Compilers.Z)))))
+      | ident_Z_min : (ident (type.arrow (type.base (pattern.base.type.type_base Compilers.Z)) (type.arrow (type.base (pattern.base.type.type_base Compilers.Z)) (type.base (pattern.base.type.type_base Compilers.Z)))))
+      | ident_Z_max : (ident (type.arrow (type.base (pattern.base.type.type_base Compilers.Z)) (type.arrow (type.base (pattern.base.type.type_base Compilers.Z)) (type.base (pattern.base.type.type_base Compilers.Z)))))
+      | ident_Z_bneg : (ident (type.arrow (type.base (pattern.base.type.type_base Compilers.Z)) (type.base (pattern.base.type.type_base Compilers.Z))))
+      | ident_Z_lnot_modulo : (ident (type.arrow (type.base (pattern.base.type.type_base Compilers.Z)) (type.arrow (type.base (pattern.base.type.type_base Compilers.Z)) (type.base (pattern.base.type.type_base Compilers.Z)))))
+      | ident_Z_truncating_shiftl : (ident (type.arrow (type.base (pattern.base.type.type_base Compilers.Z)) (type.arrow (type.base (pattern.base.type.type_base Compilers.Z)) (type.arrow (type.base (pattern.base.type.type_base Compilers.Z)) (type.base (pattern.base.type.type_base Compilers.Z))))))
+      | ident_Z_mul_split : (ident (type.arrow (type.base (pattern.base.type.type_base Compilers.Z)) (type.arrow (type.base (pattern.base.type.type_base Compilers.Z)) (type.arrow (type.base (pattern.base.type.type_base Compilers.Z)) (type.base (pattern.base.type.prod (pattern.base.type.type_base Compilers.Z) (pattern.base.type.type_base Compilers.Z)))))))
+      | ident_Z_add_get_carry : (ident (type.arrow (type.base (pattern.base.type.type_base Compilers.Z)) (type.arrow (type.base (pattern.base.type.type_base Compilers.Z)) (type.arrow (type.base (pattern.base.type.type_base Compilers.Z)) (type.base (pattern.base.type.prod (pattern.base.type.type_base Compilers.Z) (pattern.base.type.type_base Compilers.Z)))))))
+      | ident_Z_add_with_carry : (ident (type.arrow (type.base (pattern.base.type.type_base Compilers.Z)) (type.arrow (type.base (pattern.base.type.type_base Compilers.Z)) (type.arrow (type.base (pattern.base.type.type_base Compilers.Z)) (type.base (pattern.base.type.type_base Compilers.Z))))))
+      | ident_Z_add_with_get_carry : (ident (type.arrow (type.base (pattern.base.type.type_base Compilers.Z)) (type.arrow (type.base (pattern.base.type.type_base Compilers.Z)) (type.arrow (type.base (pattern.base.type.type_base Compilers.Z)) (type.arrow (type.base (pattern.base.type.type_base Compilers.Z)) (type.base (pattern.base.type.prod (pattern.base.type.type_base Compilers.Z) (pattern.base.type.type_base Compilers.Z))))))))
+      | ident_Z_sub_get_borrow : (ident (type.arrow (type.base (pattern.base.type.type_base Compilers.Z)) (type.arrow (type.base (pattern.base.type.type_base Compilers.Z)) (type.arrow (type.base (pattern.base.type.type_base Compilers.Z)) (type.base (pattern.base.type.prod (pattern.base.type.type_base Compilers.Z) (pattern.base.type.type_base Compilers.Z)))))))
+      | ident_Z_sub_with_get_borrow : (ident (type.arrow (type.base (pattern.base.type.type_base Compilers.Z)) (type.arrow (type.base (pattern.base.type.type_base Compilers.Z)) (type.arrow (type.base (pattern.base.type.type_base Compilers.Z)) (type.arrow (type.base (pattern.base.type.type_base Compilers.Z)) (type.base (pattern.base.type.prod (pattern.base.type.type_base Compilers.Z) (pattern.base.type.type_base Compilers.Z))))))))
+      | ident_Z_zselect : (ident (type.arrow (type.base (pattern.base.type.type_base Compilers.Z)) (type.arrow (type.base (pattern.base.type.type_base Compilers.Z)) (type.arrow (type.base (pattern.base.type.type_base Compilers.Z)) (type.base (pattern.base.type.type_base Compilers.Z))))))
+      | ident_Z_add_modulo : (ident (type.arrow (type.base (pattern.base.type.type_base Compilers.Z)) (type.arrow (type.base (pattern.base.type.type_base Compilers.Z)) (type.arrow (type.base (pattern.base.type.type_base Compilers.Z)) (type.base (pattern.base.type.type_base Compilers.Z))))))
+      | ident_Z_rshi : (ident (type.arrow (type.base (pattern.base.type.type_base Compilers.Z)) (type.arrow (type.base (pattern.base.type.type_base Compilers.Z)) (type.arrow (type.base (pattern.base.type.type_base Compilers.Z)) (type.arrow (type.base (pattern.base.type.type_base Compilers.Z)) (type.base (pattern.base.type.type_base Compilers.Z)))))))
+      | ident_Z_cc_m : (ident (type.arrow (type.base (pattern.base.type.type_base Compilers.Z)) (type.arrow (type.base (pattern.base.type.type_base Compilers.Z)) (type.base (pattern.base.type.type_base Compilers.Z)))))
+      | ident_Z_combine_at_bitwidth : (ident (type.arrow (type.base (pattern.base.type.type_base Compilers.Z)) (type.arrow (type.base (pattern.base.type.type_base Compilers.Z)) (type.arrow (type.base (pattern.base.type.type_base Compilers.Z)) (type.base (pattern.base.type.type_base Compilers.Z))))))
+      | ident_Z_cast : (ident (type.arrow (type.base (pattern.base.type.type_base Compilers.Z)) (type.base (pattern.base.type.type_base Compilers.Z))))
+      | ident_Z_cast2 : (ident (type.arrow (type.base (pattern.base.type.prod (pattern.base.type.type_base Compilers.Z) (pattern.base.type.type_base Compilers.Z))) (type.base (pattern.base.type.prod (pattern.base.type.type_base Compilers.Z) (pattern.base.type.type_base Compilers.Z)))))
+      | ident_Some : (forall A : pattern.base.type.type base, ident (type.arrow (type.base A) (type.base (pattern.base.type.option A))))
+      | ident_None : (forall A : pattern.base.type.type base, ident (type.base (pattern.base.type.option A)))
+      | ident_option_rect : (forall A P : pattern.base.type.type base, ident (type.arrow (type.arrow (type.base A) (type.base P)) (type.arrow (type.arrow (type.base pattern.base.type.unit) (type.base P)) (type.arrow (type.base (pattern.base.type.option A)) (type.base P)))))
+      | ident_Build_zrange : (ident (type.arrow (type.base (pattern.base.type.type_base Compilers.Z)) (type.arrow (type.base (pattern.base.type.type_base Compilers.Z)) (type.base (pattern.base.type.type_base Compilers.zrange)))))
+      | ident_zrange_rect : (forall P : pattern.base.type.type base, ident (type.arrow (type.arrow (type.base (pattern.base.type.type_base Compilers.Z)) (type.arrow (type.base (pattern.base.type.type_base Compilers.Z)) (type.base P))) (type.arrow (type.base (pattern.base.type.type_base Compilers.zrange)) (type.base P))))
+      | ident_fancy_add : (ident (type.arrow (type.base (pattern.base.type.prod (pattern.base.type.prod (pattern.base.type.type_base Compilers.Z) (pattern.base.type.type_base Compilers.Z)) (pattern.base.type.prod (pattern.base.type.type_base Compilers.Z) (pattern.base.type.type_base Compilers.Z)))) (type.base (pattern.base.type.prod (pattern.base.type.type_base Compilers.Z) (pattern.base.type.type_base Compilers.Z)))))
+      | ident_fancy_addc : (ident (type.arrow (type.base (pattern.base.type.prod (pattern.base.type.prod (pattern.base.type.type_base Compilers.Z) (pattern.base.type.type_base Compilers.Z)) (pattern.base.type.prod (pattern.base.type.prod (pattern.base.type.type_base Compilers.Z) (pattern.base.type.type_base Compilers.Z)) (pattern.base.type.type_base Compilers.Z)))) (type.base (pattern.base.type.prod (pattern.base.type.type_base Compilers.Z) (pattern.base.type.type_base Compilers.Z)))))
+      | ident_fancy_sub : (ident (type.arrow (type.base (pattern.base.type.prod (pattern.base.type.prod (pattern.base.type.type_base Compilers.Z) (pattern.base.type.type_base Compilers.Z)) (pattern.base.type.prod (pattern.base.type.type_base Compilers.Z) (pattern.base.type.type_base Compilers.Z)))) (type.base (pattern.base.type.prod (pattern.base.type.type_base Compilers.Z) (pattern.base.type.type_base Compilers.Z)))))
+      | ident_fancy_subb : (ident (type.arrow (type.base (pattern.base.type.prod (pattern.base.type.prod (pattern.base.type.type_base Compilers.Z) (pattern.base.type.type_base Compilers.Z)) (pattern.base.type.prod (pattern.base.type.prod (pattern.base.type.type_base Compilers.Z) (pattern.base.type.type_base Compilers.Z)) (pattern.base.type.type_base Compilers.Z)))) (type.base (pattern.base.type.prod (pattern.base.type.type_base Compilers.Z) (pattern.base.type.type_base Compilers.Z)))))
+      | ident_fancy_mulll : (ident (type.arrow (type.base (pattern.base.type.prod (pattern.base.type.type_base Compilers.Z) (pattern.base.type.prod (pattern.base.type.type_base Compilers.Z) (pattern.base.type.type_base Compilers.Z)))) (type.base (pattern.base.type.type_base Compilers.Z))))
+      | ident_fancy_mullh : (ident (type.arrow (type.base (pattern.base.type.prod (pattern.base.type.type_base Compilers.Z) (pattern.base.type.prod (pattern.base.type.type_base Compilers.Z) (pattern.base.type.type_base Compilers.Z)))) (type.base (pattern.base.type.type_base Compilers.Z))))
+      | ident_fancy_mulhl : (ident (type.arrow (type.base (pattern.base.type.prod (pattern.base.type.type_base Compilers.Z) (pattern.base.type.prod (pattern.base.type.type_base Compilers.Z) (pattern.base.type.type_base Compilers.Z)))) (type.base (pattern.base.type.type_base Compilers.Z))))
+      | ident_fancy_mulhh : (ident (type.arrow (type.base (pattern.base.type.prod (pattern.base.type.type_base Compilers.Z) (pattern.base.type.prod (pattern.base.type.type_base Compilers.Z) (pattern.base.type.type_base Compilers.Z)))) (type.base (pattern.base.type.type_base Compilers.Z))))
+      | ident_fancy_rshi : (ident (type.arrow (type.base (pattern.base.type.prod (pattern.base.type.prod (pattern.base.type.type_base Compilers.Z) (pattern.base.type.type_base Compilers.Z)) (pattern.base.type.prod (pattern.base.type.type_base Compilers.Z) (pattern.base.type.type_base Compilers.Z)))) (type.base (pattern.base.type.type_base Compilers.Z))))
+      | ident_fancy_selc : (ident (type.arrow (type.base (pattern.base.type.prod (pattern.base.type.prod (pattern.base.type.type_base Compilers.Z) (pattern.base.type.type_base Compilers.Z)) (pattern.base.type.type_base Compilers.Z))) (type.base (pattern.base.type.type_base Compilers.Z))))
+      | ident_fancy_selm : (ident (type.arrow (type.base (pattern.base.type.prod (pattern.base.type.type_base Compilers.Z) (pattern.base.type.prod (pattern.base.type.prod (pattern.base.type.type_base Compilers.Z) (pattern.base.type.type_base Compilers.Z)) (pattern.base.type.type_base Compilers.Z)))) (type.base (pattern.base.type.type_base Compilers.Z))))
+      | ident_fancy_sell : (ident (type.arrow (type.base (pattern.base.type.prod (pattern.base.type.prod (pattern.base.type.type_base Compilers.Z) (pattern.base.type.type_base Compilers.Z)) (pattern.base.type.type_base Compilers.Z))) (type.base (pattern.base.type.type_base Compilers.Z))))
+      | ident_fancy_addm : (ident (type.arrow (type.base (pattern.base.type.prod (pattern.base.type.prod (pattern.base.type.type_base Compilers.Z) (pattern.base.type.type_base Compilers.Z)) (pattern.base.type.type_base Compilers.Z))) (type.base (pattern.base.type.type_base Compilers.Z))))
       .
 
-      Definition package : @GoalType.package base.type.base Compilers.ident.
-      Proof. Time Tactic.make_package Classes.exprInfo Classes.exprExtraInfo Compilers.ident Raw.ident.ident ident.ident. Defined.
+      Definition package : @GoalType.package Compilers.base Compilers.ident.
+      Proof. Time Tactic.make_package Compilers.exprInfo Compilers.exprExtraInfo Compilers.ident Raw.ident.ident ident.ident. Defined.
     End ident.
   End pattern.
 End Compilers.
